Started Deriving the canonicals
Although the project used to build it would throw an "Axiom not realized" error. Although these axioms aren't directly used they unfortunately still need to be realized.

Shims/Util.ml
@@ -1,0 +1,70 @@
+open String
+open Datatypes
+
+(* let printAddrList ls = 
+  List.iter (fun x -> Printf.printf "Address:\t (%s,%i)\n" x.ip x.port) ls *)
+
+(* let printHelp (msg: procMessage)= 
+  match msg with
+ | ConnectMsg -> "ConnectMsg"
+ | AddrMsg ls -> "AddrMsg"
+ | _ -> "Somthing Else" *)
+
+let rec add n m =
+  match n with
+  | O -> m
+  | S p -> S (add p m)
+
+(** val mul : nat -> nat -> nat **)
+
+let rec mul n m =
+  match n with
+  | O -> O
+  | S p -> add m (mul p m)
+
+let int_natlike_rec = fun fO fS ->
+ let rec loop acc i = if i <= 0 then acc else loop (fS acc) (i-1)
+ in loop fO
+
+let nat_of_int =
+  int_natlike_rec O (fun x -> S x)
+
+let int_of_nat =
+  let rec loop acc = function
+  | O -> acc
+  | S n0 -> loop (succ acc) n0
+  in loop 0
+
+let nat_of_string s = nat_of_int (int_of_string s)
+let string_of_nat n = string_of_int (int_of_nat n)
+
+let ip_of_string s = 
+  let parts = split_on_char '.' s in 
+  Printf.printf "%s, %s, %s, %s" (List.nth parts 0) (List.nth parts 1) (List.nth parts 2) (List.nth parts 3);
+  (((nat_of_string (List.nth parts 0), nat_of_string (List.nth parts 1)), nat_of_string (List.nth parts 2)), nat_of_string (List.nth parts 3))
+
+let raw_bytes_of_int (x : int) : bytes =
+  let buf = Bytes.make 4 '\x00' in
+  Bytes.set buf 0 (char_of_int (x land 0xff));
+  Bytes.set buf 1 (char_of_int ((x lsr 8) land 0xff));
+  Bytes.set buf 2 (char_of_int ((x lsr 16) land 0xff));
+  Bytes.set buf 3 (char_of_int ((x lsr 24) land 0xff));
+  buf
+
+let int_of_raw_bytes (buf : bytes) : int =
+   (int_of_char (Bytes.get buf 0)) lor
+  ((int_of_char (Bytes.get buf 1)) lsl 8) lor
+  ((int_of_char (Bytes.get buf 2)) lsl 16) lor
+  ((int_of_char (Bytes.get buf 3)) lsl 24)
+
+let getIP = function
+    | (_,(x,_)) -> Some x
+    | _ -> None
+
+let getPort = function
+    | (_,(_,x)) -> Some x
+    | _ -> None
+
+let getName = function
+    | (x,(_,_)) -> Some x
+    | _ -> None
