Shims/test.ml
@@ -1,3 +1,48 @@
 open Protocol
+open Datatypes
+(* open Util *)
+open Canonicals
+  
+let me : coq_Address ref = ref {ip = (((O,O),O),O); port=O}
+let nodes : coq_Address list ref = ref []
 
-let _ = ()
+(* let usage msg =
+  print_endline msg;
+  Printf.printf "%s usage:\n" Sys.argv.(0);
+  Printf.printf "    %s [OPTIONS] <CLUSTER>\n" (Array.get Sys.argv 0);
+  print_endline "where:";
+  print_endline "    CLUSTER   is a list of pairs of IP_ADDR PORT,";
+  print_endline "              giving all the nodes in the system.";
+  print_endline "              The first pair given is taken as  .";
+  print_endline "              the local node and treated as such.";
+  print_newline ();
+  print_endline "Options are as follows:";
+  print_endline "    -me <NAME>        the identity of this node (required)";
+  exit 1
+
+let rec parse_args = function
+  | [] -> ()
+  | "-nodes" :: ip :: port :: args ->
+      begin
+        me := {ip = (((O,O),O),O); port = O};
+        parse_args args
+      end
+  | ip :: port :: args -> begin
+      nodes := {ip = (((O,O),O),O); port = O} :: !nodes;
+      parse_args args
+    end
+  | arg :: args ->
+      usage ("Unknown argument " ^ arg)
+
+let main () = 
+  let args = List.tl (Array.to_list Sys.argv) in
+  parse_args (args);
+  (* let lstate = {nodes = !nodes; me = !me} in 
+    setup lstate;
+    Runner.node_run ();
+    closeSockets (); *)
+    () *)
+
+let _ = print_endline "test"
+  (* Printf.printf "main %s\n"  (string_of_float (Unix.time ())); *)
+  (* main () *)
