Structures/Canonicals.v
@@ -1,5 +1,5 @@
 From mathcomp.ssreflect
-Require Import ssrnat eqtype choice fintype.
+Require Import ssreflect ssrnat ssrfun eqtype choice fintype.
 
 From fcsl
 Require Import ordtype.
@@ -7,10 +7,10 @@ Require Import ordtype.
 Section Params.
     Parameter Hash: Type.
     Parameter VProof : Type.
-    
+
     Structure Address: Type := mkAddr {
-        ip:nat*nat*nat*nat;
-        port:nat
+        ip:'I_1024*'I_1024*'I_1024*'I_1024;
+        port:'I_1024
     }.
 
     Structure Transaction:Type := mkTx {
@@ -21,7 +21,6 @@ Section Params.
 End Params.
 
 Section Canonicals.
-Search "eqType".
     Definition VProof_eqMixin : Equality.mixin_of VProof. Admitted.
     Canonical VProof_eqType := EqType VProof VProof_eqMixin.
 
@@ -30,8 +29,44 @@ Search "eqType".
 
     Definition Hash_ordMixin : Ordered.mixin_of Hash_eqType. Admitted.
     Canonical Hash_ordType := OrdType Hash Hash_ordMixin.
+    
+    (* Address
+    Definition prod_of_address e :=
+    let: mkAddr ipv4 portNum := e in (ipv4, portNum).
 
-    Definition addr_eq (a b: Address):bool := andb (ip a == ip b) (port a == port b).
+    Definition address_of_prod p :=
+    let: (ipv4, portNum) := p in mkAddr ipv4 portNum.
+
+    Lemma prod_of_addressK : cancel prod_of_address address_of_prod.
+    Proof. by case. Qed.
+
+    Definition address_eqMixin := CanEqMixin prod_of_addressK.
+    Canonical Address_eqType := Eval hnf in EqType Address address_eqMixin.
+    Definition address_choiceMixin := CanChoiceMixin prod_of_addressK.
+    Canonical Address_choiceType := Eval hnf in ChoiceType Address address_choiceMixin.
+    Definition address_countMixin := CanCountMixin prod_of_addressK.
+    Canonical Address_countType := Eval hnf in CountType Address address_countMixin.
+    Definition address_finMixin := CanFinMixin prod_of_addressK.
+    Canonical Address_finType := Eval hnf in FinType Address address_finMixin. *)
+
+(*     
+    (* Transaction *)
+    Definition prod_of_transaction e :=
+    let: mkTx source destination val := e in (source, destination, val).
+
+    Definition transaction_of_prod p :=
+    let: (source, destination, val) := p in mkTx source destination val.
+
+    Lemma prod_of_transactionK : cancel prod_of_transaction transaction_of_prod.
+    Proof. by case. Qed.
+
+    Definition transaction_eqMixin := CanEqMixin prod_of_transactionK.
+    Canonical Transaction_eqType := Eval hnf in EqType Transaction transaction_eqMixin. *)
+
+End Canonicals.
+
+
+Definition addr_eq (a b: Address):bool := andb (ip a == ip b) (port a == port b).
 
     Lemma eq_addrP : Equality.axiom addr_eq. 
     Admitted.
@@ -51,9 +86,10 @@ Search "eqType".
     Definition Address_finMixin : Finite.mixin_of Addr_countType. Admitted.
     Canonical Address_finType := Eval hnf in FinType Address Address_finMixin.
 
+
+ 
     Definition trans_eq (a b:Transaction):bool := ((source a) == (source b)) && ((destination a) == (destination b)) && ((val a) == (val b)).
     Lemma eq_transP : Equality.axiom trans_eq. Admitted.
-
 
     (* Proof.
         case => sa da ma [sb] db mb; rewrite/trans_eq/=.
@@ -65,7 +101,3 @@ Search "eqType".
 
     Canonical Transaction_eqMixin := Eval hnf in EqMixin eq_transP.
     Canonical Transaction_eqType := Eval hnf in EqType Transaction Transaction_eqMixin.
-End Canonicals.
-
-
- 
