Extraction/Extraction.v
@@ -1,8 +1,11 @@
 From Toychain
-Require Import Protocol Network.
+Require Import Protocol Network Forests.
 Require Import ExtrOcamlBasic.
 
 Extraction Inline ssrbool.SimplPred.
+Extract Constant Timestamp => "float".
+(* Extract Constant Hash => "string".
+Extract Constant VProof => "string". *)
 Cd "Extraction".
     Cd "Extracted".
         Separate Extraction procMsg procInt initWorld.
