Makefile
@@ -2,6 +2,7 @@ all: default
 
 default: Makefile.coq
 	$(MAKE) -f Makefile.coq
+	ocamlbuild -tag safe_string -libs unix -I Extraction/Extracted -I Shims Shims/test.d.byte
 
 quick: Makefile.coq
 	$(MAKE) -f Makefile.coq quick
@@ -12,6 +13,10 @@ install: Makefile.coq
 clean: Makefile.coq
 	$(MAKE) -f Makefile.coq cleanall
 	rm -f Makefile.coq Makefile.coq.conf
+
+	# Added to remove extracted files
+	rm -rf Extraction/Extracted/*
+	rm -rf _build
 
 Makefile.coq: _CoqProject
 	coq_makefile -f _CoqProject -o Makefile.coq
