Shims/run.sh
@@ -1,0 +1,20 @@
+#!/usr/bin/env bash
+
+make clean; make && ocamlbuild -tag debug -tag safe_string -libs unix -I Extraction/Extracted -I Shims Shims/test.d.byte
+
+if ! [ -x ./test.d.byte ]
+then
+    echo 'test not found!'
+    echo 'Run `make test` first.'
+    exit 1
+fi
+
+lsof -ti:9001 | xargs kill
+lsof -ti:9002 | xargs kill
+lsof -ti:9003 | xargs kill
+
+(./test.d.byte -nodes 127.0.0.1 9001 127.0.0.1 9002 & ) >node1.log 2>&1
+
+(./test.d.byte -nodes 127.0.0.1 9002 127.0.0.1 9003 & ) >node2.log 2>&1
+
+./test.d.byte -nodes 127.0.0.1 9003| tee node3.log 2>&1
